wip

src/Std/Data/Iterators/Lemmas/Consumers/Monadic/Collect.lean
@@ -8,7 +8,7 @@ import Init.Data.Array.Lemmas
 import Std.Data.Iterators.Consumers.Monadic.Collect
 import Std.Data.Iterators.Lemmas.Monadic.Basic
 import Std.Data.Iterators.Producers
-import Std.Data.Iterators.Lemmas.Equivalence.Basic
+import Std.Data.Iterators.Lemmas.Equivalence.Advanced
 
 namespace Std.Iterators
 
@@ -160,167 +160,12 @@ end Consumers
 
 section Equivalence
 
-def IterStep.bundle [Iterator α m β] [Monad m] [LawfulMonad m]
-    (step : IterStep (IterM (α := α) m β) β) :
-    IterStep (Quot (ItEquiv m β)) β :=
-  step.mapIterator (Quot.mk (ItEquiv m β) ∘ BundledIterM.ofIterM)
-
-def IterM.QuotStep [Iterator α m β] [Monad m] [LawfulMonad m]
-    (it : IterM (α := α) m β) :=
-  Quot (fun (s₁ s₂ : it.Step) => s₁.1.bundle = s₂.1.bundle)
-
-def IterM.QuotStep.bundle [Iterator α m β] [Monad m] [LawfulMonad m]
-    {it : IterM (α := α) m β} : it.QuotStep → IterStep (Quot (ItEquiv m β)) β :=
-  Quot.lift (fun s => s.1.bundle) (by intro s t; exact id)
-
-open Classical in
-noncomputable def of? [Iterator α m β] [Monad m] [LawfulMonad m] (it : IterM (α := α) m β)
-    (step : IterStep (Quot (ItEquiv m β)) β) : Option it.QuotStep :=
-  if h : ∃ step' : it.QuotStep, step'.bundle = step then
-    some h.choose
-  else
-    none
-
-theorem bind_comp_aux {m} [Monad m] [LawfulMonad m] {f : α → β} {g : β → m γ} {x : m α} :
-    x >>= (g ∘ f) = (f <$> x) >>= g := by
-  simp?
-  rfl
-
-theorem exists_equiv_step [Iterator α₁ m β] [Iterator α₂ m β] [Monad m] [LawfulMonad m]
-    {ita : IterM (α := α₁) m β} {itb : IterM (α := α₂) m β}
-    (h : HItEquiv ita itb) (s : ita.Step) :
-    ∃ s' : itb.Step, s.1.bundle = s'.1.bundle := by
-  rw [HItEquiv, ItEquiv] at h
-  replace h := congrArg (CodensityT.run fun s => pure (of? ita s)) h
-  replace h := congrArg PostconditionT.Property h
-  simp [CodensityT.run_map, CodensityT.run_lift, bind, PostconditionT.bind,
-    BundledIterM.ofIterM] at h
-  rw [funext_iff] at h
-  specialize h (some <| Quot.mk _ s)
-  rw [eq_iff_iff] at h
-  replace h := h.1 ⟨s.1, s.2, ?_⟩
-  · rcases h with ⟨s', hs', h⟩
-    refine ⟨⟨s', hs'⟩, sorry⟩
-  · simp [BundledIterM.ofIterM, of?]
-    refine ⟨?_, ?_⟩
-    · exact ⟨Quot.mk _ s, rfl⟩
-    · generalize (Iff.mpr _) = hex
-      generalize hs' : (hex _).choose = s'
-      replace hex := hex.choose_spec
-      rw [hs'] at hex
-      rcases s'.exists_rep with ⟨s', h⟩
-      rw [← h]
-      rw [← h, IterM.QuotStep.bundle] at hex
-      simp at hex
-      apply Quot.sound
-      simp [hex]
-      rfl
-
-open Classical in
-noncomputable def IterM.QuotStep.uniqueMap [Iterator α₁ m β] [Iterator α₂ m β] [Monad m] [LawfulMonad m]
-    {ita : IterM (α := α₁) m β} {itb : IterM (α := α₂) m β}
-    (h : HItEquiv ita itb) : ita.QuotStep → itb.QuotStep := by
-  refine Quot.lift ?_ ?_
-  · intro s₁
-    have := exists_equiv_step h s₁
-    exact Quot.mk _ this.choose
-  · intro s₁ s₁' hs
-    simp
-    apply Quot.sound
-    have hs₁ := (exists_equiv_step h s₁).choose_spec
-    have hs₁' := (exists_equiv_step h s₁').choose_spec
-    rw [← hs₁, ← hs₁', hs]
-
-theorem IterM.QuotStep.uniqueMap_eq_id [Iterator α m β] [Monad m] [LawfulMonad m]
-    {it : IterM (α := α) m β} :
-    uniqueMap (HItEquiv.refl it) = id := by
-  simp only [uniqueMap]
-  ext s
-  rcases s.exists_rep with ⟨s, rfl⟩
-  simp
-  apply Quot.sound
-  exact (exists_equiv_step (HItEquiv.refl it) s).choose_spec.symm
-
-theorem temp {α₁ α₂ : Type w} {m : Type w → Type w'} [Monad m] [LawfulMonad m]
-    [Iterator α₁ m β] [Iterator α₂ m β]
-    {ita : IterM (α := α₁) m β} {itb : IterM (α := α₂) m β} (h : HItEquiv ita itb) :
-    ((BundledIterM.ofIterM itb).iterator.step' >>=
-        (fun s => pure (of? ita s)) ∘ IterStep.mapIterator (Quot.mk (ItEquiv m β) ∘ BundledIterM.ofIterM)).run =
-      (some ∘ IterM.QuotStep.uniqueMap h.symm ∘ Quot.mk _) <$> itb.step := by
-  simp [PostconditionT.run, Bind.bind, PostconditionT.bind, IterM.step', BundledIterM.ofIterM]
-  conv =>
-    lhs; lhs; ext s;
-    rw [of?, dif_pos ⟨IterM.QuotStep.uniqueMap h.symm (Quot.mk _ s), sorry⟩]
-  congr
-  rw [funext_iff]
-  intro s
-  simp
-  have h : ∃ step' : ita.QuotStep, step'.bundle = IterStep.mapIterator (Quot.mk (ItEquiv m β) ∘ BundledIterM.ofIterM) s.val := sorry
-  have := h.choose_spec
-  sorry
-
-theorem HItEquiv.step_eq {α₁ α₂ : Type w} {m : Type w → Type w'} [Monad m] [LawfulMonad m]
-    [Iterator α₁ m β] [Iterator α₂ m β]
-    {ita : IterM (α := α₁) m β} {itb : IterM (α := α₂) m β} (h : HItEquiv ita itb) :
-    (Quot.mk _ : _ → ita.QuotStep) <$> ita.step =
-      IterM.QuotStep.uniqueMap h.symm <$> (Quot.mk _ : _ → itb.QuotStep) <$> itb.step := by
-  have he := h
-  simp [HItEquiv, ItEquiv, funext_iff] at h
-  have h := congrArg (CodensityT.run fun s => pure (of? ita s)) h
-  simp [CodensityT.run_map, CodensityT.run_lift] at h
-  replace h := congrArg PostconditionT.run h
-  have := temp he (α₁ := α₁) (α₂ := α₂) (m := m) (ita := ita) (itb := itb)
-  rw [temp he, temp (HItEquiv.refl ita)] at h
-  simp only [comp_map] at h
-  replace h := congrArg ((fun x => Option.elim x sorry id) <$> ·) h
-  simp at h
-  simp [← h, IterM.QuotStep.uniqueMap_eq_id]
-
-theorem HItEquiv.step_congr {α₁ α₂ : Type w} {m : Type w → Type w'} [Monad m] [LawfulMonad m]
-    [Iterator α₁ m β] [Iterator α₂ m β]
-    {ita : IterM (α := α₁) m β} {itb : IterM (α := α₂) m β} (h : HItEquiv ita itb)
-    {f : _ → m γ} {g : _ → m γ}
-    (hfg : ∀ s₁ s₂, s₁.1.bundle = s₂.1.bundle → f s₁ = g s₂) :
-    (ita.step >>= f) = (itb.step >>= g) := by
-  let flift : ita.QuotStep → m γ := by
-    refine Quot.lift ?_ ?_
-    · exact f
-    · intro s₁ s₁' h''
-      have hs₁ := (exists_equiv_step h s₁)
-      have hs₁' := (exists_equiv_step h s₁')
-      let s₂ := hs₁.choose
-      have hfg₁ := hfg s₁ s₂ hs₁.choose_spec
-      have hfg₂ := hfg s₁' s₂ (h'' ▸ hs₁.choose_spec)
-      rw [hfg₁, hfg₂]
-  have hf : f = flift ∘ Quot.mk _ := rfl
-  let glift : itb.QuotStep → m γ := by
-    refine Quot.lift ?_ ?_
-    · exact g
-    · intro s₁ s₁' h''
-      replace h : HItEquiv itb ita := h.symm
-      have hs₁ := (exists_equiv_step h s₁)
-      have hs₁' := (exists_equiv_step h s₁')
-      let s₂ := hs₁.choose
-      have hfg₁ := hfg s₂ s₁ hs₁.choose_spec.symm
-      have hfg₂ := hfg s₂ s₁' (h'' ▸ hs₁.choose_spec.symm)
-      rw [← hfg₁, ← hfg₂]
-  have hg : g = glift ∘ Quot.mk _ := rfl
-  rw [hf, hg, bind_comp_aux, bind_comp_aux]
-  simp only [step_eq h, map_eq_pure_bind, bind_assoc]
-  apply bind_congr
-  intro step
-  simp
-  sorry
-
-
-theorem HItEquiv.toList_eq {α₁ α₂ : Type w} {m : Type w → Type w'} [Monad m] [LawfulMonad m]
+theorem HItEquivM.toListRev_eq [Monad m] [LawfulMonad m]
     [Iterator α₁ m β] [Iterator α₂ m β] [Finite α₁ m] [Finite α₂ m]
-    [IteratorCollect α₁ m m] [LawfulIteratorCollect α₁ m m]
-    [IteratorCollect α₂ m m] [LawfulIteratorCollect α₂ m m]
-    {ita : IterM (α := α₁) m β} {itb : IterM (α := α₂) m β} (h : HItEquiv ita itb) :
-    ita.toList = itb.toList := by
+    {ita : IterM (α := α₁) m β} {itb : IterM (α := α₂) m β} (h : HItEquivM ita itb) :
+    ita.toListRev = itb.toListRev := by
   induction ita using IterM.inductSteps generalizing itb with | step ita ihy ihs =>
-  rw [IterM.toList_eq_match_step, IterM.toList_eq_match_step]
+  rw [IterM.toListRev_eq_match_step, IterM.toListRev_eq_match_step]
   apply h.step_congr
   intro s₁ s₂ h
   simp only [IterStep.bundle] at h
@@ -335,6 +180,22 @@ theorem HItEquiv.toList_eq {α₁ α₂ : Type w} {m : Type w → Type w'} [Mona
     apply ihs ‹_›
     exact ItEquiv.exact _ _ h
   · simp
+
+theorem HItEquivM.toList_eq {α₁ α₂ : Type w} {m : Type w → Type w'} [Monad m] [LawfulMonad m]
+    [Iterator α₁ m β] [Iterator α₂ m β] [Finite α₁ m] [Finite α₂ m]
+    [IteratorCollect α₁ m m] [LawfulIteratorCollect α₁ m m]
+    [IteratorCollect α₂ m m] [LawfulIteratorCollect α₂ m m]
+    {ita : IterM (α := α₁) m β} {itb : IterM (α := α₂) m β} (h : HItEquivM ita itb) :
+    ita.toList = itb.toList := by
+  simp only [← IterM.reverse_toListRev, toListRev_eq h]
+
+theorem HItEquivM.toArray_eq [Monad m] [LawfulMonad m]
+    [Iterator α₁ m β] [Iterator α₂ m β] [Finite α₁ m] [Finite α₂ m]
+    [IteratorCollect α₁ m m] [LawfulIteratorCollect α₁ m m]
+    [IteratorCollect α₂ m m] [LawfulIteratorCollect α₂ m m]
+    {ita : IterM (α := α₁) m β} {itb : IterM (α := α₂) m β} (h : HItEquivM ita itb) :
+    ita.toArray = itb.toArray := by
+  simp only [← IterM.toArray_toList, toList_eq h]
 
 end Equivalence
 
